src/go_lang/examples/logging.v
@@ -1,0 +1,16 @@
+From iris.proofmode Require Import tactics.
+From iris.program_logic Require Export weakestpre.
+From Perennial.go_lang Require Export lang.
+From Perennial.go_lang Require Export ffi.disk.
+From Perennial.go_lang Require Import proofmode notation.
+
+Existing Instances disk_op disk_model disk_semantics disk_interp.
+
+Coercion Var' (s: string) : expr := Var s.
+
+Definition init (sz: u64): val :=
+  λ: <>,
+  let: "hdr" := AllocN #4096 #(LitByte 0) in
+  EncodeInt #0 "hdr";;
+  EncodeInt #(LitInt sz) ("hdr" +ₗ #8);;
+  ExternalOp Write (#0, "sz_buf").
